CertiGC/GCGraph.v
@@ -109,19 +109,19 @@ Proof.
 Qed.
 
 Lemma MSS_max_wordsize_signed_range: forall n,
-    0 <= n <= MAX_SPACE_SIZE -> Ptrofs.min_signed <= WORD_SIZE * n <= Ptrofs.max_signed.
+    0 <= n < MAX_SPACE_SIZE -> Ptrofs.min_signed <= WORD_SIZE * n <= Ptrofs.max_signed.
 Proof.
   intros. destruct H. split.
   - unfold WORD_SIZE. transitivity 0. 2: lia. rewrite Z.le_lteq. left.
     apply Ptrofs.min_signed_neg.
-  -  
-    apply Z.le_trans with (WORD_SIZE * MAX_SPACE_SIZE); 
-    unfold WORD_SIZE.
-    1: lia.
-    unfold MAX_SPACE_SIZE.
-    unfold Ptrofs.max_signed, Ptrofs.half_modulus, Ptrofs.modulus, Ptrofs.wordsize,
-    Wordsize_Ptrofs.wordsize.
-    destruct Archi.ptr64 eqn:?; first [now inversion Heqb | simpl; lia].
+  - 
+  rewrite Z.lt_le_pred in H0. rewrite Z.le_lteq. left.
+  apply Z.le_lt_trans with (WORD_SIZE * Z.pred MAX_SPACE_SIZE).
+  unfold WORD_SIZE. 1: lia.
+  unfold MAX_SPACE_SIZE. rewrite Z.mul_pred_r.
+  unfold Ptrofs.max_signed, Ptrofs.half_modulus, Ptrofs.modulus, Ptrofs.wordsize,
+  Wordsize_Ptrofs.wordsize.
+  destruct Archi.ptr64 eqn:?; first [now inversion Heqb | simpl; lia].
 Qed.
 
 Definition VType: Type := nat * nat.  (* generation number, block-number within generation *)
@@ -257,19 +257,19 @@ Record space: Type :=
     total_space: Z;
     space_sh: share;
     space_order: 0 <= used_space <= total_space;
-    space_upper_bound: total_space <= MAX_SPACE_SIZE;
+    space_upper_bound: total_space < MAX_SPACE_SIZE;
   }.
 
 Definition null_space: space.
 Proof.
   refine (Build_space nullval 0 0 emptyshare _ _).
   - split; apply Z.le_refl.
-  - unfold MAX_SPACE_SIZE. intro Hx; inv Hx.
+  - unfold MAX_SPACE_SIZE. vm_compute; reflexivity.
 Defined.
 
 #[export] Instance space_inhabitant: Inhabitant space := null_space.
 
-Lemma total_space_tight_range: forall sp, 0 <= total_space sp <= MAX_SPACE_SIZE.
+Lemma total_space_tight_range: forall sp, 0 <= total_space sp < MAX_SPACE_SIZE.
 Proof.
   intros. split.
   - destruct (space_order sp). transitivity (used_space sp); assumption.
@@ -289,7 +289,7 @@ Lemma used_space_signed_range: forall sp,
     Ptrofs.min_signed <= WORD_SIZE * used_space sp <= Ptrofs.max_signed.
 Proof.
   intros. apply MSS_max_wordsize_signed_range. destruct (space_order sp). split.
-  1: assumption. apply Z.le_trans with (total_space sp). 1: assumption.
+  1: assumption. apply Z.le_lt_trans with (total_space sp). 1: assumption.
   apply (proj2 (total_space_tight_range sp)).
 Qed.
 
