CertiGC/env_graph_gc.v
@@ -2,6 +2,18 @@ Require Export VST.floyd.proofauto.
 Require Export VST.floyd.library.
 Require Export CertiGraph.CertiGC.gc.
 
+(* BEGIN these patches are necessary for VST 2.12 with Coq 8.17,
+   but should no longer be necessary in VST 2.13 and beyond *)
+Ltac quick_typecheck3 ::=
+ apply quick_derives_right; go_lowerx; intros;
+ repeat apply andp_right; auto; fail.
+
+Ltac default_entailer_for_load_store ::=
+  try quick_typecheck3;
+  unfold tc_efield, tc_LR, tc_LR_strong; simpl typeof;
+  try solve [entailer!].
+(* END these patches are necessary for VST 2.12 with Coq 8.17 *)
+
 #[export] Instance CompSpecs : compspecs. make_compspecs prog. Defined.
 Definition Vprog : varspecs. mk_varspecs prog. Defined.
 
