CertiGC/verif_forward_roots.v
@@ -78,7 +78,134 @@ Proof.
     apply wand_sepcon_adjoint.
     cancel.
 Qed.
-                    
+    
+Lemma frr_Zlength: forall from to roots g roots' g',
+  forward_roots_relation from to roots g roots' g' -> Zlength roots = Zlength roots'.
+Proof.
+   induction 1; simpl; autorewrite with sublist; auto; lia. 
+Qed.
+
+Lemma Zlength_update_frames:
+ forall frs roots,
+   Zlength roots = Zlength (frames2roots frs) -> 
+   Zlength (update_frames frs roots) = Zlength frs.
+   induction frs; simpl; intros; auto.
+   destruct a; simpl in *; autorewrite with sublist. f_equal. apply IHfrs; clear IHfrs.
+   rewrite <- ZtoNat_Zlength,  <- sublist_skip by rep_lia.
+   unfold frames2roots in *.
+   simpl in *. list_solve.
+Qed.
+
+Lemma Zlength_frames2rootpairs_sublist:
+ forall k frs, 0 <= k <= Zlength frs -> 
+   Zlength (frames2rootpairs (sublist 0 k frs)) <= Zlength(frames2rootpairs frs).
+Proof.
+  intros ? ? H2.
+  revert k H2; induction frs; simpl; intros.
+      assert (k=0) by list_solve. subst k.
+      autorewrite with sublist. lia.
+      destruct (zeq k 0).
+      subst k. autorewrite with sublist. rep_lia.
+      rewrite (sublist_split 0 1) by list_solve.
+      rewrite sublist_one by rep_lia.
+      rewrite sublist_pos_cons by lia.
+      autorewrite with sublist.
+      simpl.
+
+      specialize (IHfrs (k-1) ltac:(list_solve)).
+      set (j := sublist _ _ _) in *. clearbody j.
+      unfold frames2rootpairs in *.
+      rewrite !Zlength_concat in *.
+      simpl in *. lia.
+Qed.
+
+Set Nested Proofs Allowed.
+Lemma frames_p_update_frames_sublist:
+ forall frs roots k, 
+    Zlength (frames2roots frs) = Zlength roots ->
+    0 <= k <= Zlength frs ->
+    frames_p (sublist k (Zlength frs) frs) = frames_p (sublist k (Zlength frs) (update_frames frs roots)).
+Proof.
+unfold frames2roots. 
+induction frs as [|[???]?]; intros; simpl in *; auto.
+rewrite <- ZtoNat_Zlength,  <- sublist_skip by rep_lia.
+rewrite Zlength_app in H.
+rewrite !Zlength_cons in  *.
+destruct (zeq k 0).
+- subst k.
+ rewrite !(sublist_split 0 1 (Z.succ (Zlength frs))); try list_solve.
+ rewrite Zlength_cons. rewrite Zlength_update_frames. list_solve.
+ unfold frames2roots. list_solve.
+- rewrite !(sublist_pos_cons k) by lia.
+  replace (Z.succ (Zlength frs) - 1) with (Zlength frs) by lia.
+  apply IHfrs; clear IHfrs. list_solve. lia. 
+Qed.
+
+Lemma frames_p_isptr:
+  forall sh frs,
+    frames_shell_rep sh frs |-- !! forall k, 0 <= k < Zlength frs -> isptr (frames_p (sublist k (Zlength frs) frs)).
+Proof.
+  induction frs; simpl; intros.
+  apply prop_right; list_solve.
+  sep_apply IHfrs. Intros.
+  rewrite prop_forall. apply allp_right. intro k.
+  rewrite prop_forall. apply allp_right. intro.
+  destruct (zeq k 0).
+  subst. autorewrite with sublist.
+  destruct a; simpl. Intros.
+  entailer!.
+  rewrite sublist_pos_cons by lia.
+  sep_apply IHfrs.
+  Search (sepcon (andp (prop _) _) _).
+  rewrite sepcon_andp_prop'.
+  apply derives_extract_prop; intro.
+  apply prop_right.
+  autorewrite with sublist.
+  replace (Z.succ (Zlength frs) - 1) with (Zlength frs) by lia.
+  apply H0.
+  list_solve.
+Qed.
+
+Lemma roots_weak_valid_pointer:
+     forall sh frs roots k,
+       readable_share sh ->
+       Zlength roots = Zlength (frames2rootpairs frs) ->
+       field_compatible0 (tarray int_or_ptr_type (Zlength (fr_roots (Znth k frs)))) [] (fr_root (Znth k frs)) ->
+       0 <= k < Zlength frs ->
+       forall i, 
+       0 <= i <= Zlength (fr_roots (Znth k frs)) ->
+       roots_rep sh (frames2rootpairs (update_frames frs roots)) |-- 
+         weak_valid_pointer 
+           (field_address0 (tarray int_or_ptr_type (Zlength (fr_roots (Znth k frs)))) (SUB i) 
+              (fr_root (Znth k frs))).
+Proof.
+unfold frames2rootpairs.
+induction frs as [|[???]?]; simpl; intros.
+list_solve.
+unfold roots_rep in *.
+unfold frame2rootpairs at 1 in H0.
+unfold frame2rootpairs at 1.
+rewrite <- ZtoNat_Zlength,  <- sublist_skip by rep_lia.
+rewrite <- sublist_firstn.
+rewrite iter_sepcon_app_sepcon.
+assert (Zlength fr_roots <= Zlength roots) by admit.
+destruct (zeq k 0).
+- subst k. rewrite !Znth_0_cons in *. simpl in *.
+  clear H2.
+  apply sepcon_weak_valid_pointer1; clear IHfrs.
+  rewrite iter_sepcon_frame2rootpairs'.
+  2: rewrite Zlength_sublist, Z.sub_0_r; auto; try list_solve.
+  rewrite Zlength_sublist, Z.sub_0_r by list_solve.
+  admit.
+- rewrite (Znth_pos_cons k) in * by lia. 
+  simpl in *.
+  apply sepcon_weak_valid_pointer2.
+  apply IHfrs; clear IHfrs; auto.
+  2:list_solve.
+  rewrite Zlength_app in H0.
+  rewrite Zlength_frame2rootpairs' in H0. list_solve.
+Admitted.
+
 Lemma body_forward_roots: semax_body Vprog Gprog f_forward_roots forward_roots_spec.
 Proof.
   start_function.
@@ -88,15 +215,18 @@ Proof.
   rename fr into frs.
   pose (n := Zlength frs).
   pose (nr k := (Zlength (frames2rootpairs (sublist 0 k frs)))).
-  pose (oldroots k := sublist (nr k) (Zlength roots) roots).
+  pose (oldroots k i := sublist (nr k + i) (Zlength roots) roots).
+  assert_PROP (forall k, 0 <= k < Zlength frs -> isptr (frames_p (sublist k (Zlength frs) frs))) as FRAMESP. { 
+    unfold frames_rep. sep_apply frames_p_isptr. entailer!.
+  }
   forward_while (EX k: Z,
                  EX g': LGraph, EX h': heap, EX roots': roots_t,
       PROP (0 <= k <= n;
             forward_roots_relation from to (sublist 0 (nr k) roots) g roots' g';
             heap_relation h h';
             super_compatible g' h' 
-                (update_rootpairs (frames2rootpairs frs) (map (root2val g') (roots'++oldroots k))) 
-                (roots'++oldroots k)
+                (update_rootpairs (frames2rootpairs frs) (map (root2val g') (roots'++oldroots k 0))) 
+                (roots'++oldroots k 0)
                 outlier;
             forward_condition g' h' from to)
       LOCAL (temp _frame (frames_p (sublist k n frs));
@@ -106,7 +236,7 @@ Proof.
       SEP (all_string_constants rsh gv;
            outlier_rep outlier;
            graph_rep g';
-           frames_rep sh (update_frames frs (map (root2val g') (roots'++oldroots k)));
+           frames_rep sh (update_frames frs (map (root2val g') (roots'++oldroots k 0)));
            heap_rep sh h' hp))%assert.
   - Exists 0 g h (@nil root_t).
     simpl app.
@@ -119,8 +249,18 @@ Proof.
     split. constructor. apply hr_refl. 
   - Intros.
     unfold frames_rep.
-    rewrite <- frames_shell_rep_update.
-    2:{ admit. }
+    assert (LEN: Zlength (roots' ++ oldroots k 0) = Zlength (frames2rootpairs frs)). {
+    destruct H as [_ [? _]]. red in H.
+    destruct H5 as [_ [? _]]. red in H5.
+    apply (f_equal (@Zlength val)) in H, H5.
+    rewrite !Zlength_map in H,H5.
+    apply frr_Zlength in H3.
+    pose proof (Zlength_frames2rootpairs_sublist _ _ H2).
+    rewrite Zlength_app, <- H3.
+    unfold oldroots. unfold nr.
+    list_solve.
+    }
+    rewrite <- frames_shell_rep_update by (rewrite Zlength_map; auto).
     assert (frames_shell_rep sh frs |-- valid_pointer (frames_p (sublist k n frs))). {
       clear - SH0 H2. subst n.
       revert k H2; induction frs as [ | [? ? ?] ?]; simpl; intros.
@@ -148,183 +288,195 @@ Proof.
     simpl frames_p.
     set (frs' := update_frames _ _).
     unfold frames_rep.
-           
-     
-    sep_apply (isolate_frame sh frs' k).
-    admit.
-   Intros.
-   unfold frs' at 2.
-   rewrite frame_root_address_same by admit.
-   rewrite frame_root_address_eq by admit.
-   forward.
-  forward_loop (EX i: Z, EX g' : LGraph, EX t_info': thread_info, EX roots' : roots_t,
-     PROP (forward_roots_loop from to 
-              (nat_inc_list (length (frames2roots frames0) + Z.to_nat i)) roots g roots' g';
-           thread_info_relation t_info t_info';
-           super_compatible (g', t_info', roots') outlier;
-           forward_condition g' t_info' from to)
-     LOCAL (temp _frame (frames_adr frames');
-            temp _curr (field_address0 (tarray int_or_ptr_type (Zlength s)) (SUB i) r);
-            temp _limit  (field_address0 (tarray int_or_ptr_type (Zlength s)) (SUB Zlength s) r);
-            temp _from_start (gen_start g' from);
-            temp _from_limit (limit_address g' t_info' from);
-            temp _next (next_address t_info' to))
-     SEP (all_string_constants rsh gv;
-          outlier_rep outlier;
-          graph_rep g';
-          ti_rep sh t_info ti;
-          data_at sh (Tstruct _stack_frame noattr)
-            (field_address0 (tarray int_or_ptr_type (Zlength s)) (SUB Zlength s) r,
-            (r, frames_adr frames')) a;
-          data_at sh (tarray int_or_ptr_type (Zlength s)) s r;
-          frames_rep sh frames';
-          (data_at sh (Tstruct _stack_frame noattr)
-            (field_address0 (tarray int_or_ptr_type (Zlength s)) (SUB Zlength s) r,
-            (r, frames_adr frames')) a
-            * data_at sh (tarray int_or_ptr_type (Zlength s)) s r
-            * frames_rep sh frames') -* frames_rep sh (ti_frames t_info');
-          heap_struct_rep sh (map space_tri (spaces (ti_heap t_info'))) (ti_heap_p t_info);
-          heap_rest_rep (ti_heap t_info')
-     ))%assert.
-   + Exists 0 g' t_info' roots'. entailer!.
-     split. change (Z.to_nat 0) with O. rewrite Nat.add_0_r. auto.
-     rewrite arr_field_address0 by (auto with field_compatible; rep_lia).
-     clear - H15; destruct H15 as [? _]; destruct r; try contradiction; simpl. normalize. 
-   + Intros i g'' t_info'' roots''.
-     forward_if.
-     *  admit.  (* true, but tedious *)
-     * forward_call (rsh, sh, gv, ti, g'', t_info'', roots'', outlier, from,
-         to, 0, (@inl _ (VType*Z) (Zlength (frames2roots frames0) + i))).
-      --  simpl firstn. entailer!. repeat f_equal.
-          admit. (* plausible *)
-      -- unfold thread_info_rep.
-         fold (ti_rep sh t_info'' ti).
-         replace (ti_rep sh t_info'' ti) with (ti_rep sh t_info ti) by admit. (* plausible *)
-         replace (ti_heap_p t_info'') with (ti_heap_p t_info) by admit. (* plausible *)
-         cancel.
-         eapply derives_trans; [apply modus_ponens_wand |].
-         cancel.
-      -- admit. (* whatever *)
-      -- Intros vret.
-         destruct vret as ((g3,t_info3),roots3). simpl fst in *. simpl snd in *.
-         forward.
-         ++ entailer!. admit. (* easy *)
-         ++ Exists (i+1) g3 t_info3 roots3.
-            entailer!.
-            ** admit.  (* some things to prove here *)
-            ** unfold thread_info_rep. fold (ti_rep sh t_info3 ti).
-               replace (ti_rep sh t_info3 ti) with (ti_rep sh t_info ti) by admit. (* plausible *)
-               replace (ti_heap_p t_info3) with (ti_heap_p t_info) by admit. (* plausible *)
-               cancel.
-               set (A := (data_at _ (Tstruct _stack_frame _) _ _ * _ * _)%logic).
-               clear H11 H22 H21 H20 H19 H18 H17.
-               Search (_ |-- _ * (_ -* _)).
-               Search tir
-               red in H16.
-               Print thread_info_relation.
-               admit. (* problematic *)
-
-              
-         set (B := (data_at _ (Tstruct _stack_frame _) _ _ * _ * _)%logic).
-         set (C := frames_rep _ _).
-         sep_apply (modus_ponens_wand B C).
-         
-         (B*C) (frames_rep sh frames'))
-
-         Search spaces thread_info_relation.
-     simpl.
-     unfold forward_p_address, frame_root_address. simpl.
-     unfold weak_valid_pointer.
-     Search weak_valid_pointer.
-     auto 50 with valid_pointer.
-     unfold sameblock.
-     simpl sameblock.
-     auto 50 with valid_pointer.
-     Search denote_tc_test_order.
-     rewrite arr_field_address0 by (auto with field_compatible; rep_lia).
-
-   assert (foo: environ->mpred) by admit.
-
-     forward_if foo.
-        Print heap_rest_rep.
-     
-     cancel.
-     
-     unfold limit_address.
-       rewrite arr_field_address0 by (auto with field_compatible; rep_lia).
-       simpl.
-     unfold field_address0. rewrite if_true. simpl. clear - H15.
-     auto with field_compat
-     destruct H15, r; try contradiction. simpl. reflexivity. auto.
-     clear - H3.
-
-  - pose proof lri_range f_info. unfold MAX_UINT in H6. subst n; lia.
-  - Exists g t_info roots. destruct H as [? [? [? ?]]]. entailer!.
-    split; [|split]; try easy. unfold nat_inc_list. simpl. constructor.
-    apply derives_refl.
-  - unfold fun_info_rep.
-    assert_PROP (force_val
-                   (if Archi.ptr64 then
-                      (sem_add_ptr_long tulong (offset_val 16 fi)
-                                        (Vlong (Int64.repr i)))
-                    else
-                      (sem_add_ptr_int tuint Unsigned (offset_val 8 fi) (vint i))) =
-                 field_address (tarray (if Archi.ptr64 then tulong else tuint)
-                                       (Zlength
-                                          (live_roots_indices f_info) + 2))
-                               [ArraySubsc (i+2)] fi). {
-      entailer!. simpl. unfold field_address. rewrite if_true; simpl.
-      1: f_equal; lia. unfold field_compatible in *. intuition. red. split; auto.
-      simpl. lia. } forward. do 2 rewrite Znth_pos_cons by lia.
-    replace (i + 2 - 1 - 1) with i by lia. apply semax_if_seq. rewrite Heqn in H6.
-    pose proof (fi_index_range _ _ (Znth_In _ _ H6)). forward_if.
-    + forward. do 2 rewrite Znth_pos_cons by lia.
-      replace (i + 2 - 1 - 1) with i by lia.
-      remember (Znth i (live_roots_indices f_info)).
-      replace_SEP 1 (fun_info_rep rsh f_info fi) by entailer.
-      assert_PROP (force_val
-                     (if Archi.ptr64 then
-                        (sem_add_ptr_long
-                           int_or_ptr_type (offset_val 24 ti) (Z2val z)) else
-                        (sem_add_ptr_int int_or_ptr_type
-                                         Unsigned (offset_val 12 ti) (Z2val z))) =
-                   field_address thread_info_type
-                                 [ArraySubsc z; StructField _args] ti). {
-        unfold thread_info_rep. Intros. entailer!. simpl. unfold Z2val.
-        first [rewrite sem_add_pi_ptr_special' |
-               rewrite sem_add_pl_ptr_special] ; auto. simpl. unfold field_address.
-        rewrite if_true. 1: simpl; rewrite offset_offset_val; reflexivity.
-        unfold field_compatible in *. simpl. unfold in_members. simpl. intuition. }
-      assert (Zlength roots' = Zlength roots) by
-          (apply frl_roots_Zlength in H8; assumption).
-      forward_call (rsh, sh, gv, fi, ti, g', t_info', f_info, roots', outlier, from,
-                    to, 0, (@inl _ (VType*Z) i)).
-      * simpl snd. apply prop_right.
-        change (Tpointer tvoid {| attr_volatile := false; attr_alignas := Some 2%N |})
-          with int_or_ptr_type.
-        change (Tpointer tvoid {| attr_volatile := false; attr_alignas := Some 3%N |})
-          with int_or_ptr_type. simpl. cbv [Archi.ptr64] in H14. rewrite H14.
-        rewrite <- Heqz. clear. intuition.
-      * intuition. red. rewrite H15, H5. split; assumption.
-      * Intros vret. destruct vret as [[g2 t_info2] roots2]. simpl fst in *.
-        simpl snd in *. simpl forward_p2forward_t in H16. Exists g2 t_info2 roots2.
-        assert (thread_info_relation t_info t_info2) by (eapply tir_trans; eauto).
-        assert (gen_start g' from = gen_start g2 from). {
-          eapply fr_gen_start; eauto. destruct H11 as [_ [_ [? _]]].
-          assumption. }
-        assert (limit_address g2 t_info2 from = limit_address g' t_info' from) by
-            (unfold limit_address; rewrite H22;
-             rewrite (proj1 (proj2 H20)); reflexivity).
-        assert (next_address t_info2 to = next_address t_info' to) by
-            (unfold next_address; rewrite (proj1 H20); reflexivity).
-        destruct H16 as [? [? [? ?]]]. entailer!.
-        replace (Z.to_nat (i + 1)) with (S (Z.to_nat i)) by
-            (rewrite Z2Nat.inj_add by lia; simpl; lia).
-        rewrite nat_inc_list_S. remember (Z.to_nat i) as n.
-        replace i with (Z.of_nat n) in * by (subst n;rewrite Z2Nat.id; lia).
-        simpl in H18. split; [apply frl_add_tail|]; easy.
-    + exfalso. try (rewrite !Int64.unsigned_repr in H13; [|rep_lia..]). rep_lia.
-  - Intros g' t_info' roots'. Exists g' t_info' roots'.
-    destruct H8 as [? [? [? ?]]]. entailer!. rewrite <- H5, ZtoNat_Zlength in H6.
-    easy.
-Qed.
+    sep_apply (frames_shell_rep_isolate sh frs' k). {
+     clear - H5 H3 H2 H H7.
+     subst frs' n.
+     destruct H as [_ [? _]]. red in H.
+     destruct H5 as [_ [H5 _]]. red in H5.
+     apply (f_equal (@Zlength val)) in H, H5.
+     rewrite !Zlength_map in H,H5.
+     apply frr_Zlength in H3.
+     rewrite Zlength_update_frames. lia.
+     rewrite Zlength_map.
+     subst oldroots. simpl. autorewrite with sublist. rewrite frames2roots_eq, Zlength_map.
+     rewrite <- H, <- H3.
+     assert (0 <= nr k <= Zlength roots); [ | list_solve].
+     unfold nr. 
+     rewrite H.
+     pose proof (Zlength_frames2rootpairs_sublist _ _ H2).
+     rep_lia.
+    }
+    set (OTHERS := _ -* _).
+    set (NEXT := frames_p (sublist _ _ _)).
+    destruct (Znth k frs') as [a r s] eqn:?H.
+    unfold frame_shell_rep.
+    Intros.
+    assert (LEN': Zlength (frames2roots frs) = Zlength (map (root2val g') (roots' ++ oldroots k 0))). {
+      apply frr_Zlength in H3. autorewrite with sublist. rewrite <- H3.
+      unfold oldroots. rewrite Z.add_0_r.     
+      rewrite frames2roots_eq.
+      destruct H as [_ [? _]]. red in H. rewrite <- H.
+      rewrite Zlength_map. 
+      assert (0 <= nr k <= Zlength roots); [ | list_solve].
+      unfold nr. 
+      pose proof (Zlength_frames2rootpairs_sublist _ _ H2). list_solve.
+    }
+    replace (fr_adr (Znth k frs)) with a.
+    2:{
+      replace a with (fr_adr (Znth k frs')) by (rewrite H8; auto).
+      clear - H2 LEN'. subst n frs'.
+      set (jj := map _ _) in *. clearbody jj.
+      clear - LEN' H2.
+      revert jj LEN' k H2; induction frs as [ | [???] ?]; simpl; intros; auto.
+      destruct (zeq k 0). subst k. autorewrite with sublist; simpl; auto.
+      rewrite <- ZtoNat_Zlength,  <- sublist_skip by rep_lia.
+      rewrite !Znth_pos_cons by lia.
+      apply IHfrs; clear IHfrs; [ | list_solve].
+      unfold frames2roots in *. simpl in *.
+      rewrite Zlength_app in LEN'. list_solve.
+    }
+    forward. forward.
+    entailer!. {
+       clear - H9.
+       unfold field_address0.
+       rewrite if_true. simpl. destruct H9, r; try contradiction; hnf; auto.
+       apply arr_field_compatible0; auto. rep_lia.
+    }
+    forward. {
+      unfold NEXT.
+      simpl tc_val.
+      entailer!.
+      subst frs'.
+      replace (Zlength _) with (Zlength frs).
+      rewrite <- frames_p_update_frames_sublist by (auto; list_solve).
+      destruct (zeq (k+1) (Zlength frs)).
+      rewrite e. autorewrite with sublist. hnf. auto.
+      apply isptr_is_pointer_or_null; apply FRAMESP; list_solve.
+      rewrite Zlength_update_frames; auto.
+    }
+    forward_loop (EX i: Z, EX g'' : LGraph, EX h'': heap, EX roots'' : roots_t,
+     PROP (0 <= i <= Zlength s;
+       forward_roots_relation from to (sublist 0 (nr k + i) roots) g roots'' g'';
+       heap_relation h' h'';
+       super_compatible g'' h'' 
+         (update_rootpairs (frames2rootpairs frs) (map (root2val g'') (roots''++oldroots k i))) 
+         (roots''++oldroots k i)
+         outlier;
+     forward_condition g'' h'' from to)
+LOCAL (temp _frame NEXT;
+       temp _limit  (field_address0 (tarray int_or_ptr_type (Zlength s)) (SUB Zlength s) r);
+       temp _curr (field_address0 (tarray int_or_ptr_type (Zlength s)) (SUB i) r);
+      temp _from_start (gen_start g'' from);
+      temp _from_limit (limit_address g'' h'' from);
+      temp _next (heap_next_address hp to))
+SEP (all_string_constants rsh gv;
+    outlier_rep outlier;
+    graph_rep g'';
+    data_at sh (Tstruct _stack_frame noattr)
+       (field_address0 (tarray int_or_ptr_type (Zlength s))
+           (SUB Zlength s) r, (r, NEXT)) a; 
+    OTHERS;
+    roots_rep sh (frames2rootpairs (update_frames frs (map (root2val g'') (roots''++oldroots k i))));
+    heap_rep sh h'' hp))%assert.
+  + Exists 0 g' h' roots'.
+    entailer!; [ split | ].
+    * apply hr_refl.
+    * unfold field_address0; simpl. rewrite if_true. normalize. auto with field_compatible.
+    * apply derives_refl.
+  + Intros i g'' h'' roots''.
+    forward_if.
+    *
+    rewrite isptr_denote_tc_test_order
+      by (unfold field_address0; rewrite if_true by auto with field_compatible;
+          destruct r, H9; try contradiction; auto).
+     unfold test_order_ptrs.
+      replace (sameblock _ _) with true
+       by (unfold field_address0; rewrite !if_true by auto with field_compatible; simpl;
+        destruct r, H9; try contradiction; simpl;
+        destruct (peq _ _); try contradiction; auto).
+      replace r with (fr_root (Znth k frs)).
+      2:{ clear - H8 LEN'.
+          subst frs'. admit.
+      }
+      replace (Zlength s) with (Zlength (fr_roots (Znth k frs))) by admit.
+      apply andp_right;
+      apply sepcon_weak_valid_pointer1; repeat apply sepcon_weak_valid_pointer2;
+      apply roots_weak_valid_pointer; auto; try rep_lia.
+      admit. admit. admit. admit. admit.
+      
+    * set (rp'' := frames2rootpairs _).
+      forward_call (rsh,sh,gv,g'',h'',hp,rp'',roots''++oldroots k i,outlier,from,to,0, @inl _ (VType*Z) i).
+      entailer!. simpl. repeat f_equal. admit.
+      rewrite update_rootpairs_frames2rootpairs in H13 by admit.
+      fold rp'' in H13. split; auto.
+      simpl. admit. (* ?? *)
+      Intros vret.
+      destruct vret as [[g3 h3] roots3].
+      simpl fst in *. simpl snd in *.
+      forward.
+      entailer!. admit.
+      Exists (i+1) g3 h3 roots3.
+      entailer!.
+      admit.
+      admit.
+    * forward.
+      Exists (k+1, g'', h'', roots'').
+      simpl fst. simpl snd.
+      assert (i=Zlength s). {
+        unfold field_address0 in H15.
+        rewrite !if_true in H15 by auto with field_compatible.
+        simpl in H15. destruct r; try (destruct H9; contradiction).
+        unfold sem_cmp_pp in H15; simpl in H15.
+        rewrite if_true in H15 by auto.
+        simpl in H15.
+        Search (Ptrofs.add _ _ = Ptrofs.add _ _).
+        rewrite !(Ptrofs.add_commut i0) in H15.
+        rewrite Ptrofs.translate_ltu in H15 by admit.
+        unfold Ptrofs.ltu in H15. if_tac in H15. inv H15.
+        rewrite !Ptrofs.unsigned_repr in H16 by admit. 
+        lia.
+      }
+      subst i. clear H15 H10.
+      unfold frames_rep. subst OTHERS NEXT.
+      unfold oldroots in H13|-*.
+      assert (NR: nr (k+1) = nr k + Zlength s) by admit.
+      rewrite NR.
+      entailer!.
+      -- clear H20 H19 H18 H17 H16 H15.
+         split; auto.
+         ++ eapply hr_trans; eassumption.
+         ++ Locate frames_p_update_frames.
+       replace (Zlength frs') with (Zlength frs).
+       apply frames_p_update_frames_sublist; [ | lia].
+       admit. admit.
+      -- unfold frame_shell_rep.
+         rewrite prop_true_andp by auto.
+         sep_apply modus_ponens_wand.
+         unfold frs'. cancel.
+         rewrite <- !frames_shell_rep_update; auto.
+         admit.
+         admit.
+ - forward.
+   Exists g' h' roots'.
+   destruct (zeq k n). 
+   2: { exfalso.
+        clear - n0 H2 HRE.
+        subst n.
+         assert (Zlength (sublist k (Zlength frs) frs) <> 0) by list_solve.
+         destruct (sublist k (Zlength frs) frs). list_solve. destruct f. simpl in HRE.
+         clear - HRE.  admit.   (* this is almost but not quite a contradiction; FIXME *)
+   }
+   subst k.
+   clear H2. subst n.
+   unfold oldroots, nr in *.
+   rewrite (sublist_same 0 (Zlength frs)) in * by reflexivity.
+   rewrite Z.add_0_r in *.
+   rewrite sublist_same in H3, H5 by admit.
+   Search (sublist _ _ _ = nil).
+   rewrite (sublist_nil' _ (Zlength (frames2rootpairs _))) by admit.
+   rewrite app_nil_r.
+   entailer!. 
+   clear H10 H9 H8 H7.
+   admit.
+Admitted.
+  
